\documentclass[letterpaper]{article}
\usepackage{lplfitch}
\renewcommand*{\lnot}{\mathord{\sim}}
\renewcommand*{\lor}{\mathord{\ \vee\ }}
\renewcommand*{\land}{\mathord{\ \&\ }}
\renewcommand*{\lif}{\mathord{\ \supset\ }}
\renewcommand*{\liff}{\mathord{\ \equiv\ }}
\newcommand*{\lprov}{\mathord{\ \vdash\ }}
\newcommand*{\lent}{\mathord{\ \models\ }}
\renewcommand*\lnoti[1]{\intro{\ \lnot} #1}
\renewcommand*\lnote[1]{\elim{\ \lnot} #1}
\renewcommand*\reit[1]{\ {\bf Reit:} #1}
\renewcommand*\landi[2]{\intro{\land} #1, #2}
\newcommand*{\lifia}{\ A/$\lif${\bf Intro}}
\newcommand*{\liffia}{\ A/$\liff${\bf Intro}}
\newcommand*{\lnotia}{\ A/$\lnot${\bf Intro}}
\newcommand*{\lnotea}{\ A/ $\lnot$ {\bf Elim}}
\newcommand*{\lorea}{\ A/$\lor${\bf Elim}}
\author{Addie Morrison}
\title{Homework 3}
\begin{document}
\maketitle

\section*{5.1}

\subsection*{Q2}

\subsubsection*{B}

Derive $\lnot B$

\fitchprf{
	\pline[1.]{B \lif \lnot B}[Assumption]
}{
	\subproof{
		\pline[2.]{B}[\lnotia]
	}{
		\pline[3.]{\lnot B}[\life{1}{2}]\\
		\pline[4.]{B}[\reit{2}]
	}
	\pline[5.]{~B}[\lnoti{2--4}]
}

\subsubsection*{D}

Derive $H \land \lnot I$

\fitchprf{
	\pline[1.]{I \land \lnot I}[Assumption]
}{
	\subproof{
		\pline[2.]{~H}[\lnotea]
	}{
		\pline[3.]{I \land \lnot I}[\reit{1}]
	}
	\pline[4.]{H}[\lnote{2--3}]\\
	\pline[5.]{\lnot I}[\lande{1}]\\
	\pline[6.]{H\land\lnot I}[\landi{4}{5}]
}

\subsubsection*{F}

Derive $A \liff C$:

\fitchprf{
	\pline[1.]{A \liff \lnot B}[Assumption]\\
	\pline[2.]{\lnot B \liff C}[Assumption]
}{
	\subproof{
		\pline[3.]{A}[\liffia]
	}{
		\pline[4.]{~B}[\liffe{1}{3}]\\
		\pline[5.]{C}[\liffe{2}{4}]
	}
	\subproof{
		\pline[6.]{C}[\liffia]
	}{
		\pline[7.]{~B}[\liffe{2}{6}]\\
		\pline[8.]{A}[\liffe{1}{7}]
	}
	\pline[10.]{A\liff}[\liffi{3--5}{6--8}]
}

\subsubsection*{H}

Derive $\lnot G$

\fitchprf{
	\pline[1.]{\lnot F \lif \lnot G}[Assumption]\\
	\pline[2.]{\lnot F \lor H}[Assumption]\\
	\pline[3.]{H \liff \lnot G}[Assumption]
}{
	\subproof{
		\pline[4.]{\lnot F}[\lorea]
	}{
		\pline[5.]{\lnot G}[\life{1}{4}]
	}
	\subproof{
		\pline[6.]{H}[\lorea]
	}{
		\pline[7.]{\lnot G}[\liffe{2}{6}]
	}
	\pline[8.]{\lnot G}[\lore{2}{4--5}{6--7}]
}

\subsubsection*{J}

Derive $\lnot (F \land G)$

\fitchprf{
	\pline[1.]{F \liff (\lnot G \land H)}[Assumption]
}{
	\subproof{
		\pline[2.]{F \land G}[\lnotia]
	}{
		\pline[3.]{F}[\lande{2}]\\
		\pline[4.]{\lnot G \land H}[\liffe{1}{3}]\\
		\pline[5.]{\lnot G}[\lande{4}]\\
		\pline[6.]{G}[\lande{2}]
	}
	\pline[7.]{\lnot (F\land G)}[\lnoti{2--6}]
}

\section*{5.3}

\subsection*{Q1.h}

Derive $E \lor C$

\fitchprf{
	\pline[1.]{\lnot A \lif \lnot B}[Assumption]\\
	\pline[2.]{A \lif C}[Assumption]\\
	\pline[3.]{B \lor D}[Assumption]\\
	\pline[4.]{D \lif E}[Assumption]
}{
	\subproof{
		\pline[5.]{D}[\lorea]
	}{
		\pline[6.]{E}[\life{4}{6}]\\
		\pline[7.]{E\lor C}[\lori{6}]
	}
	\subproof{
		\pline[8.]{B}[\lorea]
	}{
		\subproof{
			\pline[9.]{\lnot A}[\lnotea]
		}{
			\pline[10.]{\lnot B}[\life{1}{9}]
		}
		\pline[11.]{A}[\lnote{9--10}]\\
		\pline[12.]{C}[\life{2}{11}]\\
		\pline[13.]{E \lor C}[\lori{12}]
	}
	\pline[14.]{E \lor C}[\lore{3}{5--7}{8--13}]
}

\subsection*{Q2.h}

Derive: A

\fitchprf{
	\pline[1.]{\lnot B \lif A}[Assumption]\\
	\pline[2.]{C \lor \lnot B}[Assumption]\\
	\pline[3.]{\lnot C}[Assumption]
}{
	\subproof{
		\pline[4.]{\lnot B}[\lorea]
	}{
		\pline[5.]{A}[\life{1}{4}]
	}
	\subproof{
		\pline[6.]{C}[\lorea]
	}{
		\subproof{
			\pline[7.]{\lnot A}[\lnotea]
		}{
			\pline[8.]{\lnot C}[\reit{3}]\\
			\pline[9.]{C}[\reit{6}]
		}
		\pline[10.]{A}[\lnote{7--9}]
	}
	\pline[11.]{A}[\lore{2}{4--5}{6--10}]
}

\subsection*{Q3.n}

Derive $[\lnot A \lif \lnot (A \lif B)]\lif A$

\fitchprf{\pline{\emptyset}}{
	\subproof{
		\pline[1.]{\lnot A \lif \lnot (A \lif B)}[\lifia]
	}{
		\subproof{
			\pline[2.]{\lnot A}[\lnotea]
		}{
			\pline[3.]{\lnot (A \lif B)}[\life{1}{2}]\\
			\subproof{
				\pline[4.]{A}[\lifia]
			}{
				\subproof{
					\pline[5.]{\lnot B}[\lnotea]
				}{
					\pline[6.]{\lnot A}[\reit{2}]\\
					\pline[7.]{A}[\reit{4}]
				}
			\pline[8.]{B}[\lnote{5--7}]
			}
			\pline[9.]{A\lif B}[\lifi{4--8}]\\
			\pline[10.]{\lnot (A\lif B)}[\reit{3}]
		}
		\pline[11.]{A}[\lnote{2--10}]
	}
	\pline[12.]{[\lnot A \lif \lnot (A \lif B)]\lif A}[\lifi{1--11}]
}

\subsection*{Q4.b}

Derive $(A \land A) \liff (A \lor A)$

\fitchprf{\pline{\emptyset}}{
	\subproof{
		\pline[1.]{A\land A}[\liffia]
	}{
		\pline[2.]{A}[\lande{1}]\\
		\pline[3.]{A \lor A}[\lori{2}]
	}
	\subproof{
		\pline[4.]{A \lor A}[\liffia]
	}{
		\subproof{
			\pline[5.]{A}[\lorea]
		}{
			\pline[6.]{A \land A}[\landi{5}{5}]
		}
		\subproof{
			\pline[7.]{A}[\lorea]
		}{
			\pline[8.]{A \land A}[\landi{7}{7}]
		}
		\pline[9.]{A\land A}[\lore{4}{5--6}{6--7}]
	}
	\pline[10.]{(A \land A) \liff (A \lor A)}[\liffi{1--3}{4--10}]
}

\subsection*{Q5.d}

Prove that the set is inconsistant

\fitchprf{
	\pline[1.]{A}[Assumption]\\
	\pline[2.]{A\liff \lnot (A\liff A)}[Assumption]
}{
	\pline[3.]{\lnot (A\liff A)}[\liffe{1}{2}]\\
	\subproof{
		\pline[4.]{A}[\liffia]
	}{
		\pline[5.]{A}[\reit{4}]
	}
	\subproof{
		\pline[6.]{A}[\liffia]
	}{
		\pline[7.]{A}[\reit{6}]
	}
	\pline[8.]{A\liff A}[\liffi{4--5}{6--7}]\\
	\pline[9.]{\lnot (A\liff A)}[\reit[3]]
}
\end{document}
